Coq/Simplicity/Primitive.v
@@ -31,11 +31,11 @@ Record mixin (term : Ty -> Ty -> Type) := Mixin
 }.
 
 Record class (term : Ty -> Ty -> Type) := Class
-{ base :> Assertion.class term
-; ext  :> mixin term
+{ base : Assertion.class term
+; ext  : mixin term
 }.
 
-Structure Algebra := _Pack { domain :> Ty -> Ty -> Type; class_of : class domain }.
+Structure Algebra := _Pack { domain : Ty -> Ty -> Type; class_of : class domain }.
 
 Definition packager dom (p0 : mixin dom) :=
  [find a  | Assertion.domain a ~ dom | "is not a Assertion algebra" ]
@@ -45,12 +45,22 @@ Definition packager dom (p0 : mixin dom) :=
 
 Notation Pack dom p := (@packager dom p _ id _ id _ id).
 
+Module Coercions.
+Coercion domain : Algebra >-> Funclass.
+Coercion base : class >-> Assertion.class.
+Coercion ext : class >-> mixin.
+End Coercions.
+
+Module CanonicalStructures.
+Export Coercions.
 Canonical Structure toCore (alg : Algebra) : Core.Algebra :=
   Core.Pack alg (class_of alg).
 Canonical Structure toAssertion (alg : Algebra) : Assertion.Algebra :=
   Assertion.Pack alg (class_of alg).
+End CanonicalStructures.
 
 Module Combinators.
+Export CanonicalStructures.
 
 Definition prim {A B} {alg : Algebra} : Prim.t A B -> alg A B := prim (class_of alg).
 
@@ -64,8 +74,8 @@ Record mixin {alg1 alg2 : Algebra} (rel : forall {A B}, alg1 A B -> alg2 A B -> 
  }.
 
 Record class {alg1 alg2 : Algebra} (rel : forall {A B}, alg1 A B -> alg2 A B -> Prop) :=
- { base :> Assertion.Parametric.class (@rel)
- ; ext :> mixin (@rel)
+ { base : Assertion.Parametric.class (@rel)
+ ; ext : mixin (@rel)
  }.
 
 Record Rel (alg1 alg2 : Algebra) := Pack
@@ -76,6 +86,7 @@ Record Rel (alg1 alg2 : Algebra) := Pack
 End Parametric.
 
 Section Reynolds.
+Import Combinators.
 Local Coercion Parametric.rel : Parametric.Rel >-> Funclass.
 
 Definition Reynolds {A B} (x y : forall (alg : Algebra), alg A B) : Prop :=
@@ -98,7 +109,7 @@ Hint Immediate prim_Parametric : parametricity.
 
 Definition primSem M A B := Kleisli (ReaderT Prim.env M) A B.
 
-Definition PrimSem_mixin (M : CIMonadZero) : Primitive.mixin (primSem M) :=
+Definition PrimSem_mixin (M : CIMonadZero) : mixin (primSem M) :=
   {| Primitive.prim A B p := fun a e => optionZero (Prim.sem e p a)
    |}.
 
@@ -106,16 +117,137 @@ Canonical Structure CorePrimSem (M : CIMonad) : Core.Algebra :=
   Core.Pack (primSem M) (CoreSem_mixin (ReaderT_CIMonad Prim.env M)).
 Canonical Structure AssertionPrimSem (M : CIMonadZero) : Assertion.Algebra :=
   Assertion.Pack (primSem M) (AssertionSem_mixin (ReaderT_CIMonadZero Prim.env M)).
-Canonical Structure AssertionSem (M : CIMonadZero) : Primitive.Algebra :=
-  Primitive.Pack (primSem M) (PrimSem_mixin M).
+Canonical Structure PrimitivePrimSem (M : CIMonadZero) : Algebra :=
+  Pack (primSem M) (PrimSem_mixin M).
 
 Definition CommitmentRoot_Primitive_mixin : Primitive.mixin CommitmentRoot :=
  {| Primitive.prim A B p := Prim.tag p
   |}.
 
-Canonical Structure CommitmentRoot_Primitive_alg : Primitive.Algebra :=
-  Primitive.Pack CommitmentRoot CommitmentRoot_Primitive_mixin.
+Canonical Structure CommitmentRoot_Primitive_alg : Algebra :=
+  Pack CommitmentRoot CommitmentRoot_Primitive_mixin.
+
+Definition WitnessRoot_Primitive_mixin : Primitive.mixin WitnessRoot :=
+ {| Primitive.prim A B p := Prim.tag p
+  |}.
+
+Canonical Structure WitnessRoot_Primitive_alg : Algebra :=
+  Pack WitnessRoot WitnessRoot_Primitive_mixin.
 
 End Theory.
 
 End Primitive.
+
+Definition jetTag := Eval vm_compute in tag (MerkleRoot.prefix ++ ["Jet"%string]) refl_equal.
+
+Module Jet (Prim : PrimitiveSig).
+Module Primitive := Primitive Prim.
+Import Primitive.Theory.
+
+Record mixin (term : Ty -> Ty -> Type) := Mixin
+{ jet : forall {A B} (t : forall (term : Primitive.Algebra), term A B),
+          Primitive.Parametric t -> term A B
+}.
+
+Record class (term : Ty -> Ty -> Type) := Class
+{ base : Primitive.class term
+; ext  : mixin term
+}.
+
+Structure Algebra := _Pack { domain : Ty -> Ty -> Type; class_of : class domain }.
+
+Definition packager dom (p0 : mixin dom) :=
+ [find a  | Primitive.domain a ~ dom | "is not a Primitive algebra" ]
+ [find ac | Primitive.class_of a ~ ac ]
+ [find p  | p ~ p0 | "is not the right mixin" ]
+ @_Pack dom (@Class dom ac p).
+
+Notation Pack dom p := (@packager dom p _ id _ id _ id).
+
+Module Coercions.
+Coercion domain : Algebra >-> Funclass.
+Coercion base : class >-> Primitive.class.
+Coercion ext : class >-> mixin.
+End Coercions.
+
+Module CanonicalStructures.
+Export Coercions.
+Canonical Structure toCore (alg : Algebra) : Core.Algebra :=
+  Core.Pack alg (class_of alg).
+Canonical Structure toAssertion (alg : Algebra) : Assertion.Algebra :=
+  Assertion.Pack alg (class_of alg).
+Canonical Structure toPrimitive (alg : Algebra) : Primitive.Algebra :=
+  Primitive.Pack alg (class_of alg).
+End CanonicalStructures.
+
+Module Combinators.
+Export CanonicalStructures.
+
+Definition jet {A B} {alg : Algebra} : forall (t : _), Primitive.Parametric t -> alg A B :=
+  jet (class_of alg).
+
+End Combinators.
+
+Module Parametric.
+Import Combinators.
+
+Record mixin {alg1 alg2 : Algebra} (rel : forall {A B}, alg1 A B -> alg2 A B -> Prop) :=
+ { _ : forall A B (t : _) (p : Primitive.Parametric t), @rel A B (jet p) (jet p)
+ }.
+
+Record class {alg1 alg2 : Algebra} (rel : forall {A B}, alg1 A B -> alg2 A B -> Prop) :=
+ { base : Assertion.Parametric.class (@rel)
+ ; ext : mixin (@rel)
+ }.
+
+Record Rel (alg1 alg2 : Algebra) := Pack
+ { rel :> forall {A B}, alg1 A B -> alg2 A B -> Prop
+ ; class_of : class (@rel)
+ }.
+
+End Parametric.
+
+Section Reynolds.
+Import Combinators.
+Local Coercion Parametric.rel : Parametric.Rel >-> Funclass.
+
+Definition Reynolds {A B} (x y : forall (alg : Algebra), alg A B) : Prop :=
+  forall alg1 alg2 (R : Parametric.Rel alg1 alg2), R A B (x alg1) (y alg2).
+
+Definition Parametric {A B} (x : forall (alg : Algebra), alg A B) : Prop := Reynolds x x.
+End Reynolds.
+
+Module Theory.
+Export Combinators.
+Coercion Parametric.rel : Parametric.Rel >-> Funclass.
+
+Lemma jet_Parametric {alg1 alg2 : Algebra} (R : Parametric.Rel alg1 alg2)
+  {A B} {t : _} (p : Primitive.Parametric t) : R A B (jet p) (jet p).
+Proof.
+destruct R as [R [Rb []]].
+cbn; auto.
+Qed.
+Hint Resolve jet_Parametric : parametricity.
+
+Definition PrimSem_jet_mixin (M : CIMonadZero) : mixin (primSem M) :=
+  {| Jet.jet A B t p := t (PrimitivePrimSem M) |}.
+
+Canonical Structure PrimitivePrimSem (M : CIMonadZero) : Algebra :=
+  Pack (primSem M) (PrimSem_jet_mixin M).
+
+Definition CommitmentRoot_Jet_mixin : Jet.mixin CommitmentRoot :=
+ {| Jet.jet A B t p := compress_half jetTag (witnessRoot (t _))
+  |}.
+
+Canonical Structure CommitmentRoot_Jet_alg : Algebra :=
+  Pack CommitmentRoot CommitmentRoot_Jet_mixin.
+
+Definition WitnessRoot_Jet_mixin : Jet.mixin WitnessRoot :=
+ {| Jet.jet A B t p := compress_half jetTag (witnessRoot (t _))
+  |}.
+
+Canonical Structure WitenssRoot_Jet_alg : Algebra :=
+  Pack WitnessRoot WitnessRoot_Jet_mixin.
+
+End Theory.
+End Jet.
