Coq/Simplicity/Ty.v
@@ -1,3 +1,5 @@
+Set Implicit Arguments.
+
 Inductive Ty : Set :=
 | Unit : Ty
 | Sum  : Ty -> Ty -> Ty
@@ -17,3 +19,16 @@ Coercion tySem : Ty >-> Sortclass.
 
 Definition Arrow (A B : Ty) := A -> B.
 Definition Kleisli (M : Type -> Type) (A B : Ty) := A -> M B.
+
+Record tyAlg (A : Set) : Set :=
+{ unitA : A
+; sumA  : A -> A -> A
+; prodA : A -> A -> A
+}.
+
+Fixpoint tyCata A (alg : tyAlg A) (t : Ty) : A :=
+match t with
+| Unit => unitA alg
+| Sum tl tr => sumA alg (tyCata alg tl) (tyCata alg tr)
+| Prod t1 t2 => prodA alg (tyCata alg t1) (tyCata alg t2)
+end.
